caseStudy/ADT/List/Impl/LemArrayList.dfy
@@ -1,6 +1,7 @@
 include "../../../../theory/math/ExpReal.dfy"
 include "../../../../theory/math/TypeR0.dfy"
 include "../../../../theory/ComplexityR0.dfy"
+include "../../../../theory/LemComplexityR0.dfy"
 
 /******************************************************************************
   Auxiliary module for ArrayList verification
@@ -11,6 +12,7 @@ module LemArrayList {
   import opened ExpReal
   import opened TypeR0
   import opened ComplexityR0
+  import opened LemComplexityR0
 
   // Complexity analysis for Get operation  
 
@@ -41,24 +43,24 @@ module LemArrayList {
   ghost function Tinsert(N:nat, k:nat) : R0
     requires N >= k
   {
-    (N - k) as R0
+    (N - k + 1) as R0
   }
 
   ghost function Tinsert2(N:nat) : R0
   {
-    N as R0
+    (N + 1) as R0
   }  
 
   lemma lem_Insert_Tinsert2BigOlin() returns (c:R0, n0:nat) 
     ensures bigOfrom(c, n0, Tinsert2, linGrowth())
   {
-    c, n0 := 1.0, 1;
+    c, n0 := 2.0, 1;
     forall n:nat | 0 <= n0 <= n
       ensures Tinsert2(n) <= c*linGrowth()(n)
     {
       calc {
            Tinsert2(n);
-        == n as R0;
+        == (n + 1) as R0;
         <= c*n as R0;
         == { lem_expOne(n as R0); }
            c*exp(n as R0, 1.0);
@@ -66,6 +68,21 @@ module LemArrayList {
       }
     }
     assert bigOfrom(c, n0, Tinsert2, linGrowth());
+  }
+
+  // Complexity analysis for Append operation 
+
+  ghost function Tappend(N:nat) : R0
+  {
+    1.0
+  }
+
+  lemma lem_Append_TappendBigOconst() returns (c:R0, n0:nat) 
+    ensures bigOfrom(c, n0, Tappend, constGrowth())
+  {
+    lem_bigO_constGrowth(Tappend, 1.0);
+    var c':R0, n0':nat :| bigOfrom(c', n0', Tappend, constGrowth());
+    c, n0 := c', n0';
   }
 
   // Complexity analysis for Delete operation  
